src/spec/TLS13.ConnectionState.ClientCertificateVerifyEvent.fsti
@@ -1,0 +1,30 @@
+module TLS13.ConnectionState.ClientCertificateVerifyEvent
+
+module CL = TLS13.ConnectionLog
+module CVR = TLS13.ConnectionState.ClientCertificateVerifyReachability
+module M = TLS13.Messages
+
+open TLS13.Spec.ConnectionState
+
+noextract
+val contains_received_certificate_verify
+  : events:list conn_event -> Tot prop
+
+noextract
+val client_certificate_verify_event_log_invariant
+  : st:connection_state -> Tot prop
+
+val lemma_connection_state_consistent_client_certificate_verify_event_log
+  (st:connection_state)
+  : Lemma
+      (requires connection_state_consistent st)
+      (ensures client_certificate_verify_event_log_invariant st)
+
+val lemma_client_application_ready_received_certificate_verify_event
+  (st:connection_state)
+  : Lemma
+      (requires
+        connection_state_consistent st /\
+        st.cs_model.model_config.config_role == ClientEndpoint /\
+        st.cs_model.model_control == ControlApplicationData)
+      (ensures contains_received_certificate_verify st.cs_event_log)
